theories/StackMachines/Util/Enumerable.v
@@ -5,12 +5,9 @@
     (1) Saarland University, Saarbrücken, Germany
 *)
 
+Require Cantor.
 Require Import ssreflect ssrbool ssrfun.
-Require Import Arith Psatz.
-Require Import List.
-Import ListNotations.
 
-Set Default Proof Using "Type".
 Set Default Goal Selector "!".
 
 (* Enumerable X allows injection into nat *)
@@ -29,7 +26,7 @@ Proof.
   move /(f_equal of_nat). by rewrite ?enumP.
 Qed.
 
-Lemma enumarableI {X Y: Type} {enum: Enumerable X} (to_X: Y -> X) (of_X: X -> Y) : 
+Lemma enumerableI {X Y: Type} {enum: Enumerable X} (to_X: Y -> X) (of_X: X -> Y) : 
   (forall (y: Y), of_X (to_X y) = y) -> Enumerable Y.
 Proof.
   move=> cancel. exists (fun y => to_nat (to_X y)) (fun x => of_X (of_nat x)).
@@ -45,35 +42,10 @@ Proof.
   by case.
 Qed.
 
-Module nat2_Enumerable.
-
-(* bijection from nat * nat to nat *)
-Definition encode '(x, y) : nat := 
-  y + (nat_rec _ 0 (fun i m => (S i) + m) (y + x)).
-
-(* bijection from nat to nat * nat *)
-Definition decode (n : nat) : nat * nat := 
-  nat_rec _ (0, 0) (fun _ '(x, y) => if x is S x then (x, S y) else (S y, 0)) n.
-
-Lemma decode_encode {xy: nat * nat} : decode (encode xy) = xy.
-Proof.
-  move Hn: (encode xy) => n. elim: n xy Hn.
-  { by move=> [[|?] [|?]]. }
-  move=> n IH [x [|y [H]]] /=.
-  - move: x => [|x [H]] /=; first done.
-    by rewrite (IH (0, x)) /= -?H ?Nat.add_0_r.
-  - by rewrite (IH (S x, y)) /= -?H ?Nat.add_succ_r.
-Qed.
-
-Lemma encode_non_decreasing (x y: nat) : x + y <= encode (x, y).
-Proof. elim: x=> [| x IH] /=; [| rewrite Nat.add_succ_r /=]; by lia. Qed.
-
-End nat2_Enumerable.
-
 #[export] Instance nat2_Enumerable : Enumerable (nat * nat).
 Proof.
-  exists nat2_Enumerable.encode nat2_Enumerable.decode.
-  move=> ?. by apply: nat2_Enumerable.decode_encode.
+  exists Cantor.to_nat Cantor.of_nat.
+  exact: Cantor.cancel_of_to.
 Qed.
 
 #[export] Instance prod_Enumerable {X Y: Type} {enumX: Enumerable X} {enumY: Enumerable Y} : Enumerable (X * Y).
@@ -90,35 +62,4 @@ Proof.
     (fun t => match t with | inl x => to_nat (0, to_nat x) | inr y => to_nat (1, to_nat y) end)
     (fun n => match of_nat n with | (0, n) => inl (of_nat n) | (1, n) => inr (of_nat n) | _ => inl (of_nat n) end).
   by case => ?; rewrite ?enumP.
-Qed.
-
-Module list_Enumerable.
-Section list_Enumerable_Section.
-Variables (X: Type) (enumX: Enumerable X).
-
-Fixpoint encode (L: list X) : nat :=
-  if L is x :: L then 1+nat2_Enumerable.encode (1 + to_nat x, encode L) else 1+nat2_Enumerable.encode (0, 0).
-
-Fixpoint decode (i: nat) (n: nat) : list X :=
-  if i is S i then match nat2_Enumerable.decode (n-1) with | (0, _) => [] | (S n1, n2) => (of_nat n1) :: decode i n2 end else [].
-
-Opaque nat2_Enumerable.encode nat2_Enumerable.decode.
-
-Lemma decode_encode {L: list X} : decode (encode L) (encode L) = L.
-Proof.
-  suff: forall i, encode L <= i -> decode i (encode L) = L by (apply; lia).
-  move=> i. elim: i L; first by (move=> [|? L] /=; lia).
-  move=> i IH [|x L] /= ?; first done.
-  rewrite Nat.sub_0_r nat2_Enumerable.decode_encode enumP IH; last done.
-  have := nat2_Enumerable.encode_non_decreasing (S (@to_nat X enumX x)) (encode L).
-  by lia.
-Qed.
-
-End list_Enumerable_Section.
-End list_Enumerable.
-
-#[export] Instance list_Enumerable {X: Type} {enumX: Enumerable X} : Enumerable (list X).
-Proof.
-  exists (list_Enumerable.encode X enumX) (fun n => list_Enumerable.decode X enumX n n).
-  move=> ?. by apply: list_Enumerable.decode_encode.
 Qed.
