theories/StackMachines/Util/Facts.v
@@ -4,25 +4,13 @@ Require Import ssreflect ssrbool ssrfun.
 
 Set Default Goal Selector "!".
 
-(* induction principle wrt. a decreasing measure f *)
-(* example: elim /(measure_ind length) : l. *)
-Lemma measure_ind {X : Type} (f : X -> nat) (P : X -> Prop) : 
-  (forall x, (forall y, f y < f x -> P y) -> P x) -> forall (x : X), P x.
-  Proof.
-  apply : well_founded_ind.
-  apply : Wf_nat.well_founded_lt_compat. move => *. by eassumption.
-  Qed.
-Arguments measure_ind {X}.
-
-(* induction principle wrt. a decreasing measure f *)
-(* example: elim /(measure_ind length) : l. *)
+(* induction/recursion principle wrt. a decreasing measure f *)
+(* example: elim /(measure_rect length) : l. *)
 Lemma measure_rect {X : Type} (f : X -> nat) (P : X -> Type) : 
   (forall x, (forall y, f y < f x -> P y) -> P x) -> forall (x : X), P x.
 Proof.
-  apply : well_founded_induction_type.
-  apply : Wf_nat.well_founded_lt_compat. move => *. by eassumption.
+  exact: (well_founded_induction_type (Wf_nat.well_founded_lt_compat X f _ (fun _ _ => id)) P).
 Qed.
-Arguments measure_rect {X}.
 
 (* duplicates argument *)
 Lemma copy {A : Prop} : A -> A * A.
